try DLL with ADT

SlowTest/DLL-ADT.dfy
@@ -1,28 +1,18 @@
-/*
-
-If Z3 fails to verify this file, try these Dafny options:
-
-  /noNLarith /proverOpt:OPTIMIZE_FOR_BV=true /z3opt:smt.PHASE_SELECTION=0 /z3opt:smt.RESTART_STRATEGY=0 /z3opt:smt.RESTART_FACTOR=1.5 /z3opt:smt.ARITH.RANDOM_INITIAL_VALUE=true /z3opt:smt.CASE_SPLIT=1
-
-Explanation:
-
-  Dafny/Boogie sets smt.CASE_SPLIT=3, which seems good in general, but makes this file unstable.
-
-  Z3's default is smt.CASE_SPLIT=1.
-
-  There's no direct way to override the smt.CASE_SPLIT=3, but /proverOpt:OPTIMIZE_FOR_BV=true blocks it,
-
-  along with a bunch of other options (e.g. smt.PHASE_SELECTION=0);
-
-  these other options then must be restored manually, as shown above.
-
-*/
-
- 
-
 newtype{:nativeType "ulong"} uint64 = i:int | 0 <= i < 0x1_0000_0000_0000_0000
 
 datatype Option<V> = None | Some(value:V) 
+type AbInt(==)
+function method int2adt (n: int) : (r: AbInt)
+predicate AbIsZero (n: AbInt) {n == int2adt(0)}
+predicate AbNonNeg (n: AbInt) { true }
+predicate AbPos (n: AbInt) {AbNonNeg(n) && !AbIsZero(n)}
+
+function method AbLt(n: AbInt, m: AbInt) : bool
+function method AbAdd(n: AbInt, m: AbInt) : (r: AbInt)
+function method AbSub(n: AbInt, m: AbInt) : (r: AbInt)
+lemma Props_plus_and_minus ()
+  ensures forall x, y, z :: AbAdd(x, y) == z ==> AbSub(z, y) == x && AbSub(z, x) == y
+
 
 function method seq_get<A>(s:seq<A>, i:uint64):(a:A)
   requires i as int < |s|
@@ -80,36 +70,37 @@ datatype DList<A> = DList(
   nodes:seq<Node<A>>, // sequence of nodes held by the list, indexed by pointer p
   freeStack:uint64, // pointer to singly-linked stack of free nodes
   ghost s:seq<A>, // sequence of data values held by the list, indexed by integer index i
-  ghost f:seq<int>, // map index to pointer: f[i] = p (where p > 0)
-  ghost g:seq<int>  // map pointer to index: g[p] = i (where g[p] == -2 means p is unused and g[0] == -1 (sentinel))
+  ghost f:seq<AbInt>, // map index to pointer: f[i] = p (where p > 0)
+  ghost g:seq<AbInt>  // map pointer to index: g[p] = i (where g[p] == -2 means p is unused and g[0] == -1 (sentinel))
   )
 
 ghost const unused:int := -2
 ghost const sentinel:int := -1
 
 // make sure the list-seq mapping is correct.
-predicate Invs<A>(nodes:seq<Node<A>>, freeStack:uint64, s:seq<A>, f:seq<int>, g:seq<int>)
+predicate Invs<A>(nodes:seq<Node<A>>, freeStack:uint64, s:seq<A>, f:seq<AbInt>, g:seq<AbInt>)
 {
   && |f| == |s|
   && |g| == |nodes|
   && |nodes| > 0
-  && g[0] == sentinel
+  && g[0] == int2adt(sentinel)
   && 0 <= freeStack as int < |nodes|
-  && (forall i :: 0 <= i < |f| ==> 0 < f[i] < |nodes|)
-  && (forall i {:trigger g[f[i]]} :: 0 <= i < |f| ==> g[f[i]] == i)
+  && (forall i :: 0 <= i < |f| ==> AbLt(int2adt(0), f[i]) && AbLt(f[i], int2adt(|nodes|)))
+  && (forall i {:trigger g[f[i]]} :: 0 <= i < |f| ==> g[f[i]] == i) // TODO
   && (forall p :: 0 <= p < |g| ==>
-    && unused <= g[p] < |s|
+    && (AbLt(int2adt(unused), g[p]) || int2adt(unused) == g[p]) && AbLt(g[p], int2adt(|s|))
     && 0 <= nodes[p].next as int < |g|
-    && (g[p] >= 0 <==> nodes[p].data.Some?))
-  && (forall p :: 0 <= p < |g| && sentinel <= g[p] ==>
-    && (g[p] == sentinel ==> p == 0)
-    && (0 <= g[p] ==> f[g[p]] == p && nodes[p].data == Some(s[g[p]]))
+    && ((AbLt(int2adt(0), g[p]) || int2adt(0) == g[p]) <==> nodes[p].data.Some?))
+  && (forall p :: 0 <= p < |g| && 
+      (AbLt(int2adt(sentinel), g[p]) || int2adt(sentinel) == g[p]) ==>
+    && (int2adt(sentinel) == g[p] ==> p == 0)
+    && ((AbLt(int2adt(0), g[p]) || int2adt(0) == g[p]) ==> f[g[p]] == p && nodes[p].data == Some(s[g[p]])) // TODO
     && nodes[p].next as int == (
-      if g[p] + 1 < |f| then f[g[p] + 1] // nonlast.next or sentinel.next
+      if AbAdd(g[p], int2adt(1)) < int2adt(|f|) then f[g[p] + 1] // nonlast.next or sentinel.next // TODO
       else 0) // last.next == sentinel or sentinel.next == sentinel
     && nodes[p].prev as int == (
-      if g[p] > 0 then f[g[p] - 1] // nonfirst.prev
-      else if g[p] == 0 || |f| == 0 then 0 // first.prev == sentinel or sentinel.prev == sentinel
+      if AbLt(int2adt(0), g[p]) then f[g[p] - 1] // nonfirst.prev // TODO
+      else if int2adt(0) == g[p] || |f| == 0 then int2adt(0) // first.prev == sentinel or sentinel.prev == sentinel
       else f[|f| - 1]) // sentinel.prev == last
     )
 }
@@ -127,7 +118,7 @@ function Seq<A>(l:DList<A>):seq<A>
 function ValidPtr<A>(l:DList<A>, p:uint64):(b:bool)
   ensures b ==> p != 0
 {
-  0 < p as int < |l.g| && l.g[p] >= 0
+  0 < p as int < |l.g| && (AbLt(int2adt(0), l.g[p]) || l.g[p] == int2adt(0))
 }
  
 predicate MaybePtr<A>(l:DList<A>, p:uint64)
@@ -142,99 +133,99 @@ function Index<A>(l:DList<A>, p:uint64):(i:int)
   if Inv(l) && MaybePtr(l, p) then l.g[p] else 0
 }
  
-function IndexHi<A>(l:DList<A>, p:uint64):(i:int)
-  ensures Inv(l) && ValidPtr(l, p) ==> i == Index(l, p)
-  ensures Inv(l) && p == 0 ==> i == |Seq(l)|
-{
-  if Inv(l) && ValidPtr(l, p) then l.g[p] else |l.s|
-}
+// function IndexHi<A>(l:DList<A>, p:uint64):(i:int)
+//   ensures Inv(l) && ValidPtr(l, p) ==> i == Index(l, p)
+//   ensures Inv(l) && p == 0 ==> i == |Seq(l)|
+// {
+//   if Inv(l) && ValidPtr(l, p) then l.g[p] else |l.s|
+// }
  
-function method Get<A>(l:DList<A>, p:uint64):(a:A)
-  requires Inv(l)
-  requires ValidPtr(l, p)
-  ensures a == Seq(l)[Index(l, p)]
-{
-  seq_get(l.nodes, p).data.value
-}
+// function method Get<A>(l:DList<A>, p:uint64):(a:A)
+//   requires Inv(l)
+//   requires ValidPtr(l, p)
+//   ensures a == Seq(l)[Index(l, p)]
+// {
+//   seq_get(l.nodes, p).data.value
+// }
  
-function method Next<A>(l:DList<A>, p:uint64):(p':uint64)
-  requires Inv(l)
-  requires MaybePtr(l, p)
-  ensures MaybePtr(l, p')
-  ensures p == 0 && |Seq(l)| > 0 ==> Index(l, p') == 0
-  ensures p == 0 && |Seq(l)| == 0 ==> p' == 0
-  ensures p != 0 && Index(l, p) + 1 < |Seq(l)| ==> Index(l, p') == Index(l, p) + 1
-  ensures p != 0 && Index(l, p) + 1 == |Seq(l)| ==> p' == 0
-{
-  seq_get(l.nodes, p).next
-}
+// function method Next<A>(l:DList<A>, p:uint64):(p':uint64)
+//   requires Inv(l)
+//   requires MaybePtr(l, p)
+//   ensures MaybePtr(l, p')
+//   ensures p == 0 && |Seq(l)| > 0 ==> Index(l, p') == 0
+//   ensures p == 0 && |Seq(l)| == 0 ==> p' == 0
+//   ensures p != 0 && Index(l, p) + 1 < |Seq(l)| ==> Index(l, p') == Index(l, p) + 1
+//   ensures p != 0 && Index(l, p) + 1 == |Seq(l)| ==> p' == 0
+// {
+//   seq_get(l.nodes, p).next
+// }
  
-function method Prev<A>(l:DList<A>, p:uint64):(p':uint64)
-  requires Inv(l)
-  requires MaybePtr(l, p)
-  ensures MaybePtr(l, p')
-  ensures p == 0 && |Seq(l)| > 0 ==> Index(l, p') == |Seq(l)| - 1
-  ensures p == 0 && |Seq(l)| == 0 ==> p' == 0
-  ensures p != 0 && Index(l, p) > 0 ==> Index(l, p') == Index(l, p) - 1
-  ensures p != 0 && Index(l, p) == 0 == |Seq(l)| ==> p' == 0
-{
-  seq_get(l.nodes, p).prev
-}
+// function method Prev<A>(l:DList<A>, p:uint64):(p':uint64)
+//   requires Inv(l)
+//   requires MaybePtr(l, p)
+//   ensures MaybePtr(l, p')
+//   ensures p == 0 && |Seq(l)| > 0 ==> Index(l, p') == |Seq(l)| - 1
+//   ensures p == 0 && |Seq(l)| == 0 ==> p' == 0
+//   ensures p != 0 && Index(l, p) > 0 ==> Index(l, p') == Index(l, p) - 1
+//   ensures p != 0 && Index(l, p) == 0 == |Seq(l)| ==> p' == 0
+// {
+//   seq_get(l.nodes, p).prev
+// }
  
-method BuildFreeStack<A>(a:seq<Node<A>>, k:uint64) returns(b:seq<Node<A>>)
-  requires 0 < k as nat <= |a|
-  ensures |b| == |a|
-  ensures forall i :: 0 <= i < k as nat ==> b[i] == a[i]
-  ensures forall i :: k as nat <= i < |a| <= 0xffff_ffff_ffff_ffff ==> b[i] == Node(None, i as uint64 - 1, 0)
-{
-  b := a;
-  var n := k;
-  shared_seq_length_bound(b);
-  while (n < seq_length(b))
-    invariant k as int <= n as int <= |b|
-    invariant |b| == |a|
-    invariant forall i :: 0 <= i < k as nat ==> b[i] == a[i]
-    invariant forall i :: k as nat <= i < n as nat ==> b[i] == Node(None, i as uint64 - 1, 0)
-  {
-    b := seq_set(b, n, Node(None, n - 1, 0));
-    n := n + 1;
-  }
-}
+// method BuildFreeStack<A>(a:seq<Node<A>>, k:uint64) returns(b:seq<Node<A>>)
+//   requires 0 < k as nat <= |a|
+//   ensures |b| == |a|
+//   ensures forall i :: 0 <= i < k as nat ==> b[i] == a[i]
+//   ensures forall i :: k as nat <= i < |a| <= 0xffff_ffff_ffff_ffff ==> b[i] == Node(None, i as uint64 - 1, 0)
+// {
+//   b := a;
+//   var n := k;
+//   shared_seq_length_bound(b);
+//   while (n < seq_length(b))
+//     invariant k as int <= n as int <= |b|
+//     invariant |b| == |a|
+//     invariant forall i :: 0 <= i < k as nat ==> b[i] == a[i]
+//     invariant forall i :: k as nat <= i < n as nat ==> b[i] == Node(None, i as uint64 - 1, 0)
+//   {
+//     b := seq_set(b, n, Node(None, n - 1, 0));
+//     n := n + 1;
+//   }
+// }
 
-// initial_len should be the initial capacity plus 1
-method Alloc<A>(initial_len:uint64) returns(l:DList<A>)
-  requires initial_len > 0
-  ensures Inv(l)
-  ensures Seq(l) == []
-{
-  var nodes := seq_alloc<Node>(initial_len, Node(None, 0, 0));
-  nodes := BuildFreeStack(nodes, 1);
-  l := DList(nodes, initial_len - 1, [], [], seq(initial_len as nat, p => if p == 0 then sentinel else unused));
-}
+// // initial_len should be the initial capacity plus 1
+// method Alloc<A>(initial_len:uint64) returns(l:DList<A>)
+//   requires initial_len > 0
+//   ensures Inv(l)
+//   ensures Seq(l) == []
+// {
+//   var nodes := seq_alloc<Node>(initial_len, Node(None, 0, 0));
+//   nodes := BuildFreeStack(nodes, 1);
+//   l := DList(nodes, initial_len - 1, [], [], seq(initial_len as nat, p => if p == 0 then sentinel else unused));
+// }
 
-method Free<A>(l:DList<A>)
-{
-  var DList(nodes, freeStack, s, f, g) := l;
-  var _ := seq_free(nodes);
-}
+// method Free<A>(l:DList<A>)
+// {
+//   var DList(nodes, freeStack, s, f, g) := l;
+//   var _ := seq_free(nodes);
+// }
 
-method Expand<A>(l:DList<A>) returns(l':DList<A>)
-  requires Inv(l)
-  ensures Inv(l')
-  ensures l'.s == l.s
-  ensures forall x :: ValidPtr(l, x) ==> ValidPtr(l', x) && l'.g[x] == l.g[x]
-  ensures l'.freeStack != 0 && l'.nodes[l'.freeStack].data.None?
-{
-  var DList(nodes, freeStack, s, f, g) := l;
-  shared_seq_length_bound(nodes);
-  var len := seq_length(nodes);
-  shared_seq_length_bound(nodes);
-  var len' := if len < 0x7fff_ffff_ffff_ffff then len + len else len + 1;
-  nodes := SeqResize(nodes, len', Node(None, freeStack, 0));
-  nodes := BuildFreeStack(nodes, len + 1);
-  l' := DList(nodes, len' - 1, s, f, seq(|nodes|,
-    i requires 0 <= i < |nodes| => if i < |g| then g[i] else unused));
-}
+// method Expand<A>(l:DList<A>) returns(l':DList<A>)
+//   requires Inv(l)
+//   ensures Inv(l')
+//   ensures l'.s == l.s
+//   ensures forall x :: ValidPtr(l, x) ==> ValidPtr(l', x) && l'.g[x] == l.g[x]
+//   ensures l'.freeStack != 0 && l'.nodes[l'.freeStack].data.None?
+// {
+//   var DList(nodes, freeStack, s, f, g) := l;
+//   shared_seq_length_bound(nodes);
+//   var len := seq_length(nodes);
+//   shared_seq_length_bound(nodes);
+//   var len' := if len < 0x7fff_ffff_ffff_ffff then len + len else len + 1;
+//   nodes := SeqResize(nodes, len', Node(None, freeStack, 0));
+//   nodes := BuildFreeStack(nodes, len + 1);
+//   l' := DList(nodes, len' - 1, s, f, seq(|nodes|,
+//     i requires 0 <= i < |nodes| => if i < |g| then g[i] else unused));
+// }
  
 // Remove from dlist and seq
 // ~1s
@@ -246,49 +237,19 @@ method Remove<A>(l:DList<A>, p:uint64) returns(l':DList<A>)
   ensures forall x :: x != p && ValidPtr(l, x) ==>
     ValidPtr(l', x) && Index(l', x) == Index(l, x) - (if Index(l, x) < Index(l, p) then 0 else 1)
 {
-  if (*) {
-    var DList(nodes, freeStack, s, f, g) := l;
-    ghost var index := g[p];
-    ghost var s' := s[.. index] + s[index + 1 ..];
-    ghost var f' := f[.. index] + f[index + 1 ..];
-    ghost var g' := seq(|g|, x requires 0 <= x < |g| =>
-      if g[x] == index then unused else if g[x] > index then g[x] - 1 else g[x]);
-    var node := seq_get(nodes, p);
-    var node_prev := seq_get(nodes, node.prev);
-    nodes := seq_set(nodes, node.prev, node_prev.(next := node.next));
-    var node_next := seq_get(nodes, node.next);
-    nodes := seq_set(nodes, node.next, node_next.(prev := node.prev));
-    nodes := seq_set(nodes, p, Node(None, freeStack, 0));
-    l' := DList(nodes, p, s', f', g');
-  // } else if (*) {
-  //   var DList(nodes, freeStack, s, f, g) := l;
-  //   ghost var index := g[p];
-  //   ghost var s' := s[.. index] + s[index + 1 ..];
-  //   ghost var f' := f[.. index] + f[index + 1 ..];
-  //   ghost var g' := seq(|g|, x requires 0 <= x < |g| =>
-  //     if g[x] == index then unused else if g[x] > index then g[x] - 1 else g[x]);
-  //   var node := seq_get(nodes, p);
-  //   var node_prev := seq_get(nodes, node.prev);
-  //   nodes := seq_set(nodes, node.prev, node_prev.(next := node.next));
-  //   var node_next := seq_get(nodes, node.next);
-  //   nodes := seq_set(nodes, node.next, node_next.(prev := node.prev));
-  //   nodes := seq_set(nodes, p, Node(None, freeStack, 0));
-  //   l' := DList(nodes, p, s', f', g');
-  } else {
-    var DList(nodes, freeStack, s, f, g) := l;
-    ghost var index := g[p];
-    ghost var s' := s[.. index] + s[index + 1 ..];
-    ghost var f' := f[.. index] + f[index + 1 ..];
-    ghost var g' := seq(|g|, x requires 0 <= x < |g| =>
-      if g[x] == index then unused else if g[x] > index then g[x] - 1 else g[x]);
-    var node := seq_get(nodes, p);
-    var node_prev := seq_get(nodes, node.prev);
-    nodes := seq_set(nodes, node.prev, node_prev.(next := node.next));
-    var node_next := seq_get(nodes, node.next);
-    nodes := seq_set(nodes, node.next, node_next.(prev := node.prev));
-    nodes := seq_set(nodes, p, Node(None, freeStack, 0));
-    l' := DList(nodes, p, s', f', g');
-  }
+  var DList(nodes, freeStack, s, f, g) := l;
+  ghost var index := g[p];
+  ghost var s' := s[.. index] + s[index + 1 ..];
+  ghost var f' := f[.. index] + f[index + 1 ..];
+  ghost var g' := seq(|g|, x requires 0 <= x < |g| =>
+    if g[x] == index then unused else if g[x] > index then g[x] - 1 else g[x]);
+  var node := seq_get(nodes, p);
+  var node_prev := seq_get(nodes, node.prev);
+  nodes := seq_set(nodes, node.prev, node_prev.(next := node.next));
+  var node_next := seq_get(nodes, node.next);
+  nodes := seq_set(nodes, node.next, node_next.(prev := node.prev));
+  nodes := seq_set(nodes, p, Node(None, freeStack, 0));
+  l' := DList(nodes, p, s', f', g');
 }
 
 // // ~8s
